Finish proof of advance

new-semantics/coq/events/EnvSemantics.v
@@ -39,6 +39,10 @@ Inductive eval {var loc} `{Eq var} `{Eq loc} (σ : nv var loc (@val var)): tm ->
   (MOD : eval σ t1 (vl_exp σ1))
   (IMP : eval σ1 t2 v)
 : eval σ (tm_link t1 t2) v
+| ev_linkevent t1 t2 E1 v
+  (MOD : eval σ t1 (vl_ev E1))
+  (IMP : eval (nv_ev E1) t2 v)
+: eval σ (tm_link t1 t2) v
 | ev_mt
 : eval σ tm_mt (vl_exp nv_mt)
 | ev_bind x t1 t2 ℓ v1 σ2
@@ -46,6 +50,11 @@ Inductive eval {var loc} `{Eq var} `{Eq loc} (σ : nv var loc (@val var)): tm ->
   (BIND : eval (nv_floc x ℓ σ) t1 v1)
   (MOD : eval (nv_bval x (wvl_recv (close_vl 0 ℓ v1)) σ) t2 (vl_exp σ2))
 : eval σ (tm_bind x t1 t2) (vl_exp (nv_bval x (wvl_recv (close_vl 0 ℓ v1)) σ2))
+| ev_bindevent x t1 t2 ℓ v1 E2
+  (FRESH : ~ In ℓ (floc_nv σ))
+  (BIND : eval (nv_floc x ℓ σ) t1 v1)
+  (MOD : eval (nv_bval x (wvl_recv (close_vl 0 ℓ v1)) σ) t2 (vl_ev E2))
+: eval σ (tm_bind x t1 t2) (vl_exp (nv_bval x (wvl_recv (close_vl 0 ℓ v1)) (nv_ev E2)))
 .
 
 Lemma read_env_lc {var loc lang} `{Eq var} (σ : nv var loc lang) (Σ : env σ) :
@@ -76,7 +85,20 @@ Proof.
     inv IHEVAL1. repeat econstructor; eauto.
   - apply IHEVAL2. exploit IHEVAL1; eauto.
     intros LC'. inv LC'. auto.
+  - apply IHEVAL2. exploit IHEVAL1; eauto.
+    intros LC'. inv LC'. econstructor; eauto.
   - repeat constructor.
+  - assert (wvalue (wvl_recv (close_vl 0 ℓ v1))).
+    econstructor. instantiate (1 := []). ii.
+    assert (close_open_loc_eq_vl _ _ _ v1) by eapply close_open_loc_eq; rw.
+    exploit IHEVAL1; eauto. constructor; auto. intros VAL1.
+    assert (open_loc_lc_vl _ _ _ v1 VAL1) by (eapply open_loc_lc; auto).
+    rw.
+    eapply subst_loc_lc. auto.
+    repeat constructor; eauto.
+    exploit IHEVAL2.
+    constructor; auto.
+    intros VAL. inv VAL. auto.
   - assert (wvalue (wvl_recv (close_vl 0 ℓ v1))).
     econstructor. instantiate (1 := []). ii.
     assert (close_open_loc_eq_vl _ _ _ v1) by eapply close_open_loc_eq; rw.
@@ -100,15 +122,40 @@ Proof.
   try eqb2eq loc; clarify; eauto.
 Qed.
 
-Lemma read_env_subst {var loc lang} `{Eq var} `{Eq loc} (σ : nv var loc lang) :
-  forall ℓ ν w x (READ : read_env σ x = Env_wvl w),
-    read_env (subst_loc_nv ν ℓ σ) x = Env_wvl (subst_loc_wvl ν ℓ w).
+Lemma read_env_subst_loc {var loc lang} `{Eq var} `{Eq loc} (σ : nv var loc lang) x :
+ forall r ν ℓ (READ : read_env σ x = r),
+    read_env (subst_loc_nv ν ℓ σ) x =
+    match r with
+    | Env_err => Env_err
+    | Env_loc ℓ' =>
+      if eqb ℓ ℓ' then Env_loc ν else Env_loc ℓ'
+    | Env_wvl u =>
+      Env_wvl (subst_loc_wvl ν ℓ u)
+    end.
 Proof.
   induction σ; ii; ss;
   des_ifs; ss;
-  des_ifs; eqb2eq var; clarify;
-  try eqb2eq loc; clarify; eauto.
+  des_ifs; exploit IHσ; eauto;
+  ss; repeat rw; eauto.
 Qed.
+
+Lemma read_env_subst_wvl {var loc lang} `{Eq var} `{Eq loc} (σ : nv var loc lang) x :
+  forall r w ℓ (READ : read_env σ x = r),
+    read_env (subst_wvl_nv w ℓ σ) x =
+    match r with
+    | Env_err => Env_err
+    | Env_loc ℓ' =>
+      if eqb ℓ ℓ' then Env_wvl w else Env_loc ℓ'
+    | Env_wvl u =>
+      Env_wvl (subst_wvl_wvl w ℓ u)
+    end.
+Proof.
+  induction σ; ii; ss;
+  des_ifs; ss;
+  des_ifs; exploit IHσ; eauto;
+  ss; repeat rw; eauto.
+Qed.
+
 
 Lemma read_env_floc {var loc lang} `{Eq var} `{Eq loc} (σ : nv var loc lang) :
   forall w ℓ x (READ : read_env σ x = Env_wvl w) (IN : In ℓ (floc_wvl w)),
@@ -139,6 +186,15 @@ Proof.
     des; eauto.
     eapply close_floc in IN'. des.
     exploit IHEVAL1; eauto. ii; des; clarify.
+  - rewrite in_app_iff in *.
+    des; eauto.
+    eapply close_floc in IN. des.
+    exploit IHEVAL1; eauto. ii; des; clarify.
+    exploit IHEVAL2; eauto. intros IN'.
+    rewrite in_app_iff in *.
+    des; eauto.
+    eapply close_floc in IN'. des.
+    exploit IHEVAL1; eauto. ii; des; clarify.
 Qed.
 
 Lemma eval_map {var loc} `{Eq var} `{Name loc} t (σ : nv var loc (@val var)) v (EVAL : eval σ t v) :
@@ -155,22 +211,11 @@ Proof.
     econstructor; eauto.
     red. intros IN. eapply map_floc in IN; eauto.
     rrw; eauto.
-Qed.
-
-Lemma read_env_wvl {var loc lang} `{Eq var} `{Eq loc} (σ : nv var loc lang) x :
-  forall r w ℓ (READ : read_env σ x = r),
-    read_env (subst_wvl_nv w ℓ σ) x =
-    match r with
-    | Env_err => Env_err
-    | Env_loc ℓ' =>
-      if eqb ℓ ℓ' then Env_wvl w else Env_loc ℓ'
-    | Env_wvl u =>
-      Env_wvl (subst_wvl_wvl w ℓ u)
-    end.
-Proof.
-  induction σ; ii;
-  ss; des_ifs; ss; des_ifs;
-  exploit IHσ; eauto; ss; repeat rw; eauto.
+  - assert (map_close_vl _ _ _ v1) by (eapply map_close).
+    rw; eauto.
+    eapply ev_bindevent; eauto.
+    red. intros IN. eapply map_floc in IN; eauto.
+    rrw; eauto.
 Qed.
 
 Lemma eval_map_subst_loc {var loc} `{Eq var} `{Name loc} t (σ : nv var loc (@val var)) v (EVAL : eval σ t v) :
@@ -181,14 +226,16 @@ Proof.
   try solve [econstructor; eauto].
   - econstructor 1.
     eapply read_env_map with (φ := φ) in READ. ss.
-    exploit (read_env_subst _ _ _ _ x); eauto.
+    erewrite read_env_subst_loc; eauto.
+    ss.
   - assert (map_open_wvl_vl _ _ _ v) by (eapply map_open_wvl; auto).
     rw. s.
     assert (open_wvl_subst_loc_vl _ _ _ (map_vl φ v)) by (eapply open_wvl_subst_loc; auto).
     rw; eauto.
     econstructor 2.
     eapply read_env_map with (φ := φ) in READ. ss.
-    exploit (read_env_subst _ _ _ _ x); eauto.
+    erewrite read_env_subst_loc; eauto.
+    ss.
   - specialize (IHEVAL2 φ INJ ν ℓ').
     assert (map_close_vl _ _ _ v1) as RR by (eapply map_close; auto).
     rewrite RR in *; auto. clear RR.
@@ -203,6 +250,52 @@ Proof.
       (subst_loc_vl ν ℓ' (close_vl 0 ℓ'' (subst_loc_vl ℓ'' (φ ℓ) (map_vl φ v1)))) with
       (close_vl 0 ℓ'' (subst_loc_vl ν ℓ' (subst_loc_vl ℓ'' (φ ℓ) (map_vl φ v1)))) in *.
     constructor; auto.
+    { intro IN. eapply floc_subst_loc in IN. des; auto. }
+    { set (compose loc (swap id ℓ'' (φ ℓ)) φ) as φ'.
+      replace (map_nv φ σ) with (map_nv φ' σ).
+      replace (subst_loc_vl ℓ'' (φ ℓ) (map_vl φ v1)) with (map_vl φ' v1).
+      exploit (IHEVAL1 φ' _ ν).
+      subst φ'. unfold compose, swap, id.
+      ii; ss; des_ifs;
+      repeat match goal with
+      | _ => eqb2eq loc
+      | H : φ _ = φ _ |- _ => apply INJ in H
+      | _ => clarify
+      end.
+      instantiate (1 := ℓ').
+      replace (eqb ℓ' (φ' ℓ)) with false.
+      replace (φ' ℓ) with ℓ''. auto.
+      1, 2: subst φ'; unfold compose, swap, id; s; des_ifs; eqb2eq loc; clarify.
+      symmetry. apply eqb_neq. auto.
+      { assert (swap_is_subst_vl _ _ _ (map_vl φ v1)) as RR by eapply swap_is_subst.
+        specialize (RR id).
+        exploit RR; eauto. unfold oto. auto.
+        instantiate (1 := φ ℓ).
+        replace (map_vl id (map_vl φ v1)) with (map_vl φ v1) by (symmetry; eapply map_id_is_id).
+        unfold id at 2. unfold id at 2.
+        intro. rrw.
+        subst φ'. symmetry. eapply map_compose. }
+      { eapply map_ext.
+        ii. subst φ'. unfold compose, swap, id.
+        des_ifs; eqb2eq loc; clarify.
+        eapply floc_map in DOM; eauto. contradict.
+        exploit INJ; eauto. ii; clarify. } }
+    { eapply subst_loc_close; auto. }
+    { eapply subst_loc_close_eq; auto. }
+  - specialize (IHEVAL2 φ INJ ν ℓ').
+    assert (map_close_vl _ _ _ v1) as RR by (eapply map_close; auto).
+    rewrite RR in *; auto. clear RR.
+    gensym_tac (ℓ' :: φ ℓ :: ν :: floc_nv (map_nv φ σ)) ℓ''. clear Heqℓ''.
+    assert (~ In ℓ'' (floc_vl (map_vl φ v1))) as HINT.
+    { intro. apply eval_map with (φ := φ) in EVAL1; auto.
+      eapply eval_floc_dec in EVAL1; eauto. ss. des; ss. }
+    replace 
+      (close_vl 0 (φ ℓ) (map_vl φ v1)) with
+      (close_vl 0 ℓ'' (subst_loc_vl ℓ'' (φ ℓ) (map_vl φ v1))) in *.
+    replace 
+      (subst_loc_vl ν ℓ' (close_vl 0 ℓ'' (subst_loc_vl ℓ'' (φ ℓ) (map_vl φ v1)))) with
+      (close_vl 0 ℓ'' (subst_loc_vl ν ℓ' (subst_loc_vl ℓ'' (φ ℓ) (map_vl φ v1)))) in *.
+    apply ev_bindevent; auto.
     { intro IN. eapply floc_subst_loc in IN. des; auto. }
     { set (compose loc (swap id ℓ'' (φ ℓ)) φ) as φ'.
       replace (map_nv φ σ) with (map_nv φ' σ).
@@ -255,14 +348,16 @@ Proof.
   try solve [econstructor; eauto].
   - econstructor 1.
     eapply read_env_map with (φ := φ) in READ.
-    exploit (read_env_wvl _ _ _ u ℓ'); eauto.
+    erewrite read_env_subst_wvl; eauto.
+    ss.
   - assert (map_open_wvl_vl _ _ _ v) by (eapply map_open_wvl; auto).
     rw. s.
     assert (open_wvl_subst_wvl_vl _ _ _ (map_vl φ v)) by (eapply open_wvl_subst_wvl; auto).
     rw; eauto.
     econstructor 2.
     eapply read_env_map with (φ := φ) in READ.
-    exploit (read_env_wvl _ _ _ u ℓ'); eauto.
+    erewrite read_env_subst_wvl; eauto.
+    ss.
   - specialize (IHEVAL2 φ INJ u U ℓ').
     assert (map_close_vl _ _ _ v1) as RR by (eapply map_close; auto).
     rewrite RR in *; auto. clear RR.
@@ -277,6 +372,52 @@ Proof.
       (subst_wvl_vl u ℓ' (close_vl 0 ℓ'' (subst_loc_vl ℓ'' (φ ℓ) (map_vl φ v1)))) with
       (close_vl 0 ℓ'' (subst_wvl_vl u ℓ' (subst_loc_vl ℓ'' (φ ℓ) (map_vl φ v1)))) in *.
     constructor; auto.
+    { intro IN. eapply floc_subst_wvl in IN. des; auto. }
+    { set (compose loc (swap id ℓ'' (φ ℓ)) φ) as φ'.
+      replace (map_nv φ σ) with (map_nv φ' σ).
+      replace (subst_loc_vl ℓ'' (φ ℓ) (map_vl φ v1)) with (map_vl φ' v1).
+      exploit (IHEVAL1 φ' _ u U).
+      subst φ'. unfold compose, swap, id.
+      ii; ss; des_ifs;
+      repeat match goal with
+      | _ => eqb2eq loc
+      | H : φ _ = φ _ |- _ => apply INJ in H
+      | _ => clarify
+      end.
+      instantiate (1 := ℓ').
+      replace (eqb ℓ' (φ' ℓ)) with false.
+      replace (φ' ℓ) with ℓ''. auto.
+      1, 2: subst φ'; unfold compose, swap, id; s; des_ifs; eqb2eq loc; clarify.
+      symmetry. apply eqb_neq. auto.
+      { assert (swap_is_subst_vl _ _ _ (map_vl φ v1)) as RR by eapply swap_is_subst.
+        specialize (RR id).
+        exploit RR; eauto. unfold oto. auto.
+        instantiate (1 := φ ℓ).
+        replace (map_vl id (map_vl φ v1)) with (map_vl φ v1) by (symmetry; eapply map_id_is_id).
+        unfold id at 2. unfold id at 2.
+        intro. rrw.
+        subst φ'. symmetry. eapply map_compose. }
+      { eapply map_ext.
+        ii. subst φ'. unfold compose, swap, id.
+        des_ifs; eqb2eq loc; clarify.
+        eapply floc_map in DOM; eauto. contradict.
+        exploit INJ; eauto. ii; clarify. } }
+    { eapply subst_wvl_close; auto. }
+    { eapply subst_loc_close_eq; auto. }
+  - specialize (IHEVAL2 φ INJ u U ℓ').
+    assert (map_close_vl _ _ _ v1) as RR by (eapply map_close; auto).
+    rewrite RR in *; auto. clear RR.
+    gensym_tac (ℓ' :: φ ℓ :: floc_wvl u ++ floc_nv (map_nv φ σ)) ℓ''. clear Heqℓ''.
+    assert (~ In ℓ'' (floc_vl (map_vl φ v1))) as HINT.
+    { intro. apply eval_map with (φ := φ) in EVAL1; auto.
+      eapply eval_floc_dec in EVAL1; eauto. ss. des; ss. }
+    replace 
+      (close_vl 0 (φ ℓ) (map_vl φ v1)) with
+      (close_vl 0 ℓ'' (subst_loc_vl ℓ'' (φ ℓ) (map_vl φ v1))) in *.
+    replace 
+      (subst_wvl_vl u ℓ' (close_vl 0 ℓ'' (subst_loc_vl ℓ'' (φ ℓ) (map_vl φ v1)))) with
+      (close_vl 0 ℓ'' (subst_wvl_vl u ℓ' (subst_loc_vl ℓ'' (φ ℓ) (map_vl φ v1)))) in *.
+    apply ev_bindevent; auto.
     { intro IN. eapply floc_subst_wvl in IN. des; auto. }
     { set (compose loc (swap id ℓ'' (φ ℓ)) φ) as φ'.
       replace (map_nv φ σ) with (map_nv φ' σ).
