new-semantics/coq/events/Advance.v
@@ -1,0 +1,202 @@
+From Basics Require Import Basics.
+From With_events Require Import Defs.
+From With_events Require Import Syntax.
+From With_events Require Import SubstFacts.
+From With_events Require Import EnvSemantics.
+From With_events Require Import EquivSemantics.
+From With_events Require Import LinkDefs.
+From With_events Require Import LinkFacts.
+
+Section Advance.
+  Variable var : Type.
+  Variable loc : Type.
+
+  #[local] Coercion vl_ev : vnt >-> vl.
+  #[local] Coercion vl_exp : nv >-> vl.
+  #[local] Coercion wvl_v : vl >-> wvl.
+
+  Lemma advance_Eval `{Name loc} `{Eq var}
+    (σ0 σ' : nv var loc _) (Σ0 : env σ0) v' t (EVAL : Eval σ' t v') :
+    forall (σ : nv var loc _) (LINK : σ0 ⋊ σ ∋ σ'),
+      exists v, Eval σ t v /\ (σ0 ⋊ v ∋ v').
+  Proof.
+    induction EVAL; ii; ss.
+    - exploit link_read; eauto; ss.
+      intro READ'. specialize (READ' x v READ).
+      des; ss.
+      eexists; split; eauto.
+      destruct w; ss.
+      + econstructor 1; auto.
+      + econstructor 2; auto.
+    - exploit link_read; eauto; ss.
+      intro READ'. specialize (READ' x (wvl_recv v) READ).
+      des; ss.
+      eexists; split; eauto.
+      destruct w; ss.
+      + econstructor 1; auto.
+      + econstructor 2; auto.
+    - eexists; split; econstructor; eauto.
+    - exploit IHEVAL1; eauto.
+      exploit IHEVAL2; eauto.
+      intros (v2' & EVAL2' & LINK2).
+      intros (v1' & EVAL1' & LINK1).
+      destruct v1'; try solve [inv LINK1].
+      + exists (Call E v2').
+        split. eapply Ev_appevent; eauto.
+        econstructor; eauto.
+        erewrite equiv_semantics.
+        eauto.
+        eapply linked_lc_wvl in LINK; eauto. inv LINK. inv VAL.
+        eapply Eval_lc in EVAL1; auto. inv EVAL1.
+        eapply Eval_lc in EVAL2; auto.
+        repeat (constructor; auto).
+      + inv LINK1.
+        exploit IHEVAL3; eauto.
+        eapply link_bval; eauto.
+        intros (v' & EVAL' & LINK').
+        exists v'. split; try econstructor; eauto.
+    - exploit IHEVAL1; eauto.
+      exploit IHEVAL2; eauto.
+      intros (v2' & EVAL2' & LINK2).
+      intros (v1' & EVAL1' & LINK1).
+      destruct v1'; try solve [inv LINK1].
+      eexists. split.
+      eapply Ev_appevent; eauto.
+      eapply link_CallEvent; eauto.
+    - exploit IHEVAL1; eauto.
+      intros (v1' & EVAL1' & LINK1).
+      destruct v1'; try solve [inv LINK1].
+      + specialize (IHEVAL2 (nv_ev E)).
+        exploit IHEVAL2.
+        econstructor; eauto.
+        ii; des; eexists.
+        split. eapply Ev_linkevent; eauto. auto.
+      + exploit IHEVAL2; eauto; ii; des; eexists.
+        split. eapply Ev_link; eauto.
+        auto.
+    - exploit IHEVAL1; eauto.
+      intros (v1' & EVAL1' & LINK1).
+      destruct v1'; try solve [inv LINK1].
+      specialize (IHEVAL2 (nv_ev E)).
+      exploit IHEVAL2.
+      apply link_holeEvent; auto.
+      ii; des; eexists.
+      split. eapply Ev_linkevent; eauto. auto.
+    - exists nv_mt. split; econstructor; eauto.
+    - gensym_tac (L ++ floc_nv σ0 ++ floc_nv σ1 ++ floc_vl v1) ν. clear Heqν.
+      match goal with
+      | IH : forall _, ~ In _ ?L -> _, ν : loc, nIN : ~ In ν ?L |- _ =>
+        exploit (IH ν nIN);
+        first [eapply link_floc; eauto | idtac]
+      end.
+      intros (v1' & EVAL1 & LINK1).
+      eapply link_lc in LINK as Σ1. inv Σ1. inv VAL.
+      eapply Eval_lc in EVAL1 as V1; try solve [econstructor; eauto].
+      assert (forall ℓ (FREE : ~ In ℓ (floc_nv σ1)),
+        open_loc_vl 0 ℓ (close_vl 0 ν v1') = subst_loc_vl ℓ ν v1') as RR.
+      { intros.
+        assert (close_open_loc_eq_vl _ _ _ v1') by eapply close_open_loc_eq. rw.
+        assert (open_loc_lc_vl _ _ _ v1' V1) by (eapply open_loc_lc; eauto). rw.
+        reflexivity. }
+      assert (forall ℓ (FREE : ~ In ℓ (floc_nv σ1)),
+        Eval (nv_floc x ℓ σ1) t1 (open_loc_vl 0 ℓ (close_vl 0 ν v1'))).
+      { intros. apply Eval_subst_loc with (ν := ℓ) (ℓ' := ν) in EVAL1.
+        ss. rewrite eqb_refl in EVAL1.
+        assert (RR' : subst_loc_fresh_nv _ _ _ σ1) by eapply subst_loc_fresh.
+        rewrite RR' in EVAL1; eauto.
+        rewrite RR; eauto. }
+      assert (forall ℓ (FREE : ~ In ℓ (floc_nv σ1)),
+        σ0 ⋊ open_loc_vl 0 ℓ (close_vl 0 ν v1') ∋ open_loc_vl 0 ℓ v1).
+      { intros. apply link_subst_loc with (ν := ℓ) (ℓ' := ν) in LINK1; eauto.
+        assert (open_loc_subst_loc_vl _ _ _ v1) as RR' by eapply open_loc_subst_loc.
+        simpl in LINK1. rewrite RR' in LINK1. clear RR'.
+        rewrite eqb_refl in LINK1.
+        rewrite RR; eauto.
+        assert (subst_loc_fresh_nv _ _ _ σ0) as RR' by eapply subst_loc_fresh.
+        rewrite RR' in LINK1; eauto. clear RR'.
+        assert (subst_loc_fresh_vl _ _ _ v1) as RR' by eapply subst_loc_fresh.
+        rewrite RR' in LINK1; eauto. }
+      assert (σ0 ⋊ wvl_recv (close_vl 0 ν v1') ∋ wvl_recv v1).
+      { gensym_tac (floc_nv σ0 ++ floc_nv σ1 ++ floc_vl v1 ++ floc_vl (close_vl 0 ν v1')) ℓ. clear Heqℓ.
+        replace v1 with (close_vl 0 ℓ (open_loc_vl 0 ℓ v1)).
+        econstructor; eauto.
+        assert (open_loc_close_vl _ _ _ v1) by eapply open_loc_close.
+        rw.
+        eapply close_fresh; eauto. }
+      exploit (IHEVAL (nv_bval x (wvl_recv (close_vl 0 ν v1')) σ1)).
+      + econstructor; eauto.
+      + intros (v2' & EVAL2 & LINK2).
+        destruct v2'; try solve [inv LINK2].
+        * exists (nv_bval x (wvl_recv (close_vl 0 ν v1')) (nv_ev E)).
+          split. eapply Ev_bindevent; eauto.
+          econstructor; eauto.
+          econstructor; eauto.
+        * exists (nv_bval x (wvl_recv (close_vl 0 ν v1')) σ3).
+          split. econstructor; eauto.
+          econstructor; eauto.
+    - gensym_tac (L ++ floc_nv σ0 ++ floc_nv σ1 ++ floc_vl v1) ν. clear Heqν.
+      match goal with
+      | IH : forall _, ~ In _ ?L -> _, ν : loc, nIN : ~ In ν ?L |- _ =>
+        exploit (IH ν nIN);
+        first [eapply link_floc; eauto | idtac]
+      end.
+      intros (v1' & EVAL1 & LINK1).
+      eapply link_lc in LINK as Σ1. inv Σ1. inv VAL.
+      eapply Eval_lc in EVAL1 as V1; try solve [econstructor; eauto].
+      assert (forall ℓ (FREE : ~ In ℓ (floc_nv σ1)),
+        open_loc_vl 0 ℓ (close_vl 0 ν v1') = subst_loc_vl ℓ ν v1') as RR.
+      { intros.
+        assert (close_open_loc_eq_vl _ _ _ v1') by eapply close_open_loc_eq. rw.
+        assert (open_loc_lc_vl _ _ _ v1' V1) by (eapply open_loc_lc; eauto). rw.
+        reflexivity. }
+      assert (forall ℓ (FREE : ~ In ℓ (floc_nv σ1)),
+        Eval (nv_floc x ℓ σ1) t1 (open_loc_vl 0 ℓ (close_vl 0 ν v1'))).
+      { intros. apply Eval_subst_loc with (ν := ℓ) (ℓ' := ν) in EVAL1.
+        ss. rewrite eqb_refl in EVAL1.
+        assert (RR' : subst_loc_fresh_nv _ _ _ σ1) by eapply subst_loc_fresh.
+        rewrite RR' in EVAL1; eauto.
+        rewrite RR; eauto. }
+      assert (forall ℓ (FREE : ~ In ℓ (floc_nv σ1)),
+        σ0 ⋊ open_loc_vl 0 ℓ (close_vl 0 ν v1') ∋ open_loc_vl 0 ℓ v1).
+      { intros. apply link_subst_loc with (ν := ℓ) (ℓ' := ν) in LINK1; eauto.
+        assert (open_loc_subst_loc_vl _ _ _ v1) as RR' by eapply open_loc_subst_loc.
+        simpl in LINK1. rewrite RR' in LINK1. clear RR'.
+        rewrite eqb_refl in LINK1.
+        rewrite RR; eauto.
+        assert (subst_loc_fresh_nv _ _ _ σ0) as RR' by eapply subst_loc_fresh.
+        rewrite RR' in LINK1; eauto. clear RR'.
+        assert (subst_loc_fresh_vl _ _ _ v1) as RR' by eapply subst_loc_fresh.
+        rewrite RR' in LINK1; eauto. }
+      assert (σ0 ⋊ wvl_recv (close_vl 0 ν v1') ∋ wvl_recv v1).
+      { gensym_tac (floc_nv σ0 ++ floc_nv σ1 ++ floc_vl v1 ++ floc_vl (close_vl 0 ν v1')) ℓ. clear Heqℓ.
+        replace v1 with (close_vl 0 ℓ (open_loc_vl 0 ℓ v1)).
+        econstructor; eauto.
+        assert (open_loc_close_vl _ _ _ v1) by eapply open_loc_close.
+        rw.
+        eapply close_fresh; eauto. }
+      exploit (IHEVAL (nv_bval x (wvl_recv (close_vl 0 ν v1')) σ1)).
+      + econstructor; eauto.
+      + intros (v2' & EVAL2 & LINK2).
+        destruct v2'; try solve [inv LINK2].
+        exists (nv_bval x (wvl_recv (close_vl 0 ν v1')) (nv_ev E)).
+        split. eapply Ev_bindevent; eauto.
+        econstructor; eauto.
+        eapply link_holeEvent.
+        assumption.
+  Qed.
+
+  Theorem advance `{Name loc} `{Eq var}
+    (σ0 σ' : nv var loc _) (Σ0 : env σ0) v' t (EVAL : eval σ' t v') :
+    forall (σ : nv var loc _) (LINK : σ0 ⋊ σ ∋ σ'),
+      exists v, eval σ t v /\ (σ0 ⋊ v ∋ v').
+  Proof.
+    intros.
+    erewrite equiv_semantics in EVAL; eauto.
+    eapply advance_Eval in EVAL; eauto.
+    des.
+    erewrite <- equiv_semantics in EVAL; eauto.
+    eapply link_lc in LINK. inv LINK. inv VAL. auto.
+    eapply linked_lc_wvl in LINK; eauto. inv LINK. inv VAL. auto.
+  Qed.
+End Advance.
+
