new-semantics/coq/events/EquivSemantics.v
@@ -1,0 +1,331 @@
+From Basics Require Import Basics.
+From With_events Require Import Defs.
+From With_events Require Import Syntax.
+From With_events Require Import SubstFacts.
+From With_events Require Import EnvSemantics.
+
+Inductive Eval {var loc} `{Eq var} `{Eq loc} (σ : nv var loc (@val var)): tm -> (vl var loc val) -> Prop :=
+| Ev_id x v (READ : read_env σ x = Env_wvl (wvl_v v))
+: Eval σ (tm_var x) v
+| Ev_rec x v (READ : read_env σ x = Env_wvl (wvl_recv v))
+: Eval σ (tm_var x) (open_wvl_vl 0 (wvl_recv v) v)
+| Ev_fn x t
+: Eval σ (tm_lam x t) (vl_clos (v_fn x t) σ)
+| Ev_app t1 t2 x e σ1 v2 v
+  (FN : Eval σ t1 (vl_clos (v_fn x e) σ1))
+  (ARG : Eval σ t2 v2)
+  (BODY : Eval (nv_bval x (wvl_v v2) σ1) e v)
+: Eval σ (tm_app t1 t2) v
+| Ev_appevent t1 t2 E1 v2
+  (FN : Eval σ t1 (vl_ev E1))
+  (ARG : Eval σ t2 v2)
+: Eval σ (tm_app t1 t2) (vl_ev (Call E1 v2))
+| Ev_link t1 t2 σ1 v
+  (MOD : Eval σ t1 (vl_exp σ1))
+  (IMP : Eval σ1 t2 v)
+: Eval σ (tm_link t1 t2) v
+| Ev_linkevent t1 t2 E1 v
+  (MOD : Eval σ t1 (vl_ev E1))
+  (IMP : Eval (nv_ev E1) t2 v)
+: Eval σ (tm_link t1 t2) v
+| Ev_mt
+: Eval σ tm_mt (vl_exp nv_mt)
+| Ev_bind x t1 t2 L v1 σ2
+  (BIND : forall ℓ (nIN : ~ In ℓ L),
+    Eval (nv_floc x ℓ σ) t1 (open_loc_vl 0 ℓ v1))
+  (MOD : Eval (nv_bval x (wvl_recv v1) σ) t2 (vl_exp σ2))
+: Eval σ (tm_bind x t1 t2) (vl_exp (nv_bval x (wvl_recv v1) σ2))
+| Ev_bindevent x t1 t2 L v1 E2
+  (BIND : forall ℓ (nIN : ~ In ℓ L),
+    Eval (nv_floc x ℓ σ) t1 (open_loc_vl 0 ℓ v1))
+  (MOD : Eval (nv_bval x (wvl_recv v1) σ) t2 (vl_ev E2))
+: Eval σ (tm_bind x t1 t2) (vl_exp (nv_bval x (wvl_recv v1) (nv_ev E2)))
+.
+
+Lemma equiv_l {var loc} `{Eq var} `{Name loc}
+  t (σ : nv var loc (@val var)) (Σ : env σ) v (EVAL : eval σ t v) :
+  forall φ (INJ : oto φ), Eval (map_nv φ σ) t (map_vl φ v).
+Proof.
+  induction EVAL; ii; ss;
+  try solve [econstructor; eauto].
+  - apply read_env_map with (φ := φ) in READ.
+    ss. econstructor; eauto.
+  - apply read_env_map with (φ := φ) in READ.
+    ss. 
+    assert (map_open_wvl_vl _ _ _ v) by eapply map_open_wvl.
+    rw.
+    eapply Ev_rec; ss; eauto.
+  - apply eval_lc in EVAL1 as V1; eauto. inv V1.
+    apply eval_lc in EVAL2 as V2; eauto.
+    exploit IHEVAL3; eauto. repeat constructor; auto.
+    econstructor; eauto.
+  - apply eval_lc in EVAL1 as Σ1; eauto. inv Σ1.
+    econstructor; eauto.
+  - apply eval_lc in EVAL1 as Σ1; eauto. inv Σ1.
+    exploit IHEVAL2; eauto. constructor; auto.
+    eapply Ev_linkevent; eauto.
+  - apply eval_lc in EVAL1 as V1; try solve [repeat constructor; auto].
+    assert (value (map_vl φ v1)) as V1' by (eapply map_lc; auto).
+    assert (wvalue (wvl_recv (close_vl 0 ℓ v1))) as V1''.
+    econstructor. instantiate (1 := []). ii.
+    assert (close_open_loc_eq_vl _ _ _ v1) by eapply close_open_loc_eq.
+    rw.
+    assert (open_loc_lc_vl _ _ _ v1 V1) by (eapply open_loc_lc; eauto).
+    rw.
+    eapply subst_loc_lc. auto.
+    repeat match goal with
+    | IH : env ?σ -> _ |- _ =>
+      assert (env σ) as Σ' by repeat (constructor; auto);
+      specialize (IH Σ'); clear Σ'
+    end.
+    eapply Ev_bind; eauto.
+    instantiate (1 := φ ℓ :: floc_nv (map_nv φ σ)).
+    intros ℓ'' nIN. split_nIn.
+    assert (~ In ℓ'' (floc_vl (map_vl φ v1))) as HINT.
+    { intro. apply eval_map with (φ := φ) in EVAL1; auto.
+      eapply eval_floc_dec in EVAL1; eauto. ss. des; ss. }
+    assert (map_close_vl _ _ _ v1) by eapply map_close.
+    rw; eauto.
+    assert (close_open_loc_eq_vl _ _ _ (map_vl φ v1)) by eapply close_open_loc_eq.
+    rw.
+    assert (open_loc_lc_vl _ _ _ (map_vl φ v1) V1') by (eapply open_loc_lc; eauto).
+    rw.
+    set (compose loc (swap id ℓ'' (φ ℓ)) φ) as φ'.
+    replace (map_nv φ σ) with (map_nv φ' σ).
+    replace (subst_loc_vl ℓ'' (φ ℓ) (map_vl φ v1)) with (map_vl φ' v1).
+    exploit (IHEVAL1 φ').
+    + subst φ'. unfold compose, swap, id.
+      ii; ss; des_ifs;
+      repeat match goal with
+      | _ => eqb2eq loc
+      | H : φ _ = φ _ |- _ => apply INJ in H
+      | _ => clarify
+      end.
+    + replace (φ' ℓ) with ℓ''; auto.
+      subst φ'; unfold compose, swap, id; s.
+      des_ifs; eqb2eq loc; clarify.
+    + assert (swap_is_subst_vl _ _ _ (map_vl φ v1)) as RR by eapply swap_is_subst.
+      specialize (RR id).
+      exploit RR; eauto. unfold oto. auto.
+      instantiate (1 := φ ℓ).
+      replace (map_vl id (map_vl φ v1)) with (map_vl φ v1) by (symmetry; eapply map_id_is_id).
+      unfold id at 2. unfold id at 2.
+      intro. rrw.
+      subst φ'. symmetry. eapply map_compose. 
+    + eapply map_ext.
+      ii. subst φ'. unfold compose, swap, id.
+      des_ifs; eqb2eq loc; clarify.
+      eapply floc_map in DOM; eauto. contradict.
+      exploit INJ; eauto. ii; clarify.
+  - apply eval_lc in EVAL1 as V1; try solve [repeat constructor; auto].
+    assert (value (map_vl φ v1)) as V1' by (eapply map_lc; auto).
+    assert (wvalue (wvl_recv (close_vl 0 ℓ v1))) as V1''.
+    econstructor. instantiate (1 := []). ii.
+    assert (close_open_loc_eq_vl _ _ _ v1) by eapply close_open_loc_eq.
+    rw.
+    assert (open_loc_lc_vl _ _ _ v1 V1) by (eapply open_loc_lc; eauto).
+    rw.
+    eapply subst_loc_lc. auto.
+    repeat match goal with
+    | IH : env ?σ -> _ |- _ =>
+      assert (env σ) as Σ' by repeat (constructor; auto);
+      specialize (IH Σ'); clear Σ'
+    end.
+    eapply Ev_bindevent; eauto.
+    instantiate (1 := φ ℓ :: floc_nv (map_nv φ σ)).
+    intros ℓ'' nIN. split_nIn.
+    assert (~ In ℓ'' (floc_vl (map_vl φ v1))) as HINT.
+    { intro. apply eval_map with (φ := φ) in EVAL1; auto.
+      eapply eval_floc_dec in EVAL1; eauto. ss. des; ss. }
+    assert (map_close_vl _ _ _ v1) by eapply map_close.
+    rw; eauto.
+    assert (close_open_loc_eq_vl _ _ _ (map_vl φ v1)) by eapply close_open_loc_eq.
+    rw.
+    assert (open_loc_lc_vl _ _ _ (map_vl φ v1) V1') by (eapply open_loc_lc; eauto).
+    rw.
+    set (compose loc (swap id ℓ'' (φ ℓ)) φ) as φ'.
+    replace (map_nv φ σ) with (map_nv φ' σ).
+    replace (subst_loc_vl ℓ'' (φ ℓ) (map_vl φ v1)) with (map_vl φ' v1).
+    exploit (IHEVAL1 φ').
+    + subst φ'. unfold compose, swap, id.
+      ii; ss; des_ifs;
+      repeat match goal with
+      | _ => eqb2eq loc
+      | H : φ _ = φ _ |- _ => apply INJ in H
+      | _ => clarify
+      end.
+    + replace (φ' ℓ) with ℓ''; auto.
+      subst φ'; unfold compose, swap, id; s.
+      des_ifs; eqb2eq loc; clarify.
+    + assert (swap_is_subst_vl _ _ _ (map_vl φ v1)) as RR by eapply swap_is_subst.
+      specialize (RR id).
+      exploit RR; eauto. unfold oto. auto.
+      instantiate (1 := φ ℓ).
+      replace (map_vl id (map_vl φ v1)) with (map_vl φ v1) by (symmetry; eapply map_id_is_id).
+      unfold id at 2. unfold id at 2.
+      intro. rrw.
+      subst φ'. symmetry. eapply map_compose. 
+    + eapply map_ext.
+      ii. subst φ'. unfold compose, swap, id.
+      des_ifs; eqb2eq loc; clarify.
+      eapply floc_map in DOM; eauto. contradict.
+      exploit INJ; eauto. ii; clarify.
+Qed.
+
+Lemma equiv_r {var loc} `{Eq var} `{Name loc}
+  t (σ : nv var loc (@val var)) v (EVAL : Eval σ t v) :
+  eval σ t v.
+Proof.
+  induction EVAL; ii; ss;
+  try solve [econstructor; eauto].
+  - gensym_tac (floc_nv σ ++ floc_vl v1 ++ L) ℓ. clear Heqℓ.
+    assert (close_vl 0 ℓ (open_loc_vl 0 ℓ v1) = v1) as RR.
+    { assert (open_loc_close_vl _ _ _ v1) by eapply open_loc_close.
+      rw. eapply close_fresh; eauto. }
+    rewrite <- RR.
+    eapply ev_bind; eauto.
+    rw. auto.
+  - gensym_tac (floc_nv σ ++ floc_vl v1 ++ L) ℓ. clear Heqℓ.
+    assert (close_vl 0 ℓ (open_loc_vl 0 ℓ v1) = v1) as RR.
+    { assert (open_loc_close_vl _ _ _ v1) by eapply open_loc_close.
+      rw. eapply close_fresh; eauto. }
+    rewrite <- RR.
+    eapply ev_bindevent; eauto.
+    rw. auto.
+Qed.
+
+Lemma equiv_semantics {var loc} `{Eq var} `{Name loc}
+  t (σ : nv var loc (@val var)) (Σ : env σ) v :
+  eval σ t v <-> Eval σ t v.
+Proof.
+  split.
+  - intro.
+    replace σ with (map_nv id σ) by apply map_id_is_id.
+    replace v with (map_vl id v) by apply map_id_is_id.
+    eapply equiv_l; eauto. ii; ss.
+  - eapply equiv_r.
+Qed.
+
+Lemma Eval_lc {var loc} `{Eq var} `{Name loc} t (σ : nv var loc (@val var)) v (EVAL : Eval σ t v) :
+  forall (LC : env σ), value v.
+Proof.
+  induction EVAL; ii; ss; eauto.
+  - eapply read_env_lc in READ; eauto. inv READ. auto.
+  - eapply read_env_lc in READ; eauto.
+    inversion READ; clarify.
+    gensym_tac (L ++ floc_vl v) ν.
+    assert (subst_intro_vl _ _ _ v) by eapply subst_intro.
+    rw; eauto.
+    eapply subst_wvl_lc; eauto.
+  - econstructor. auto.
+  - apply IHEVAL3. econstructor.
+    econstructor. apply IHEVAL2. auto.
+    exploit IHEVAL1; eauto. intros LC'.
+    inv LC'. auto.
+  - specialize (IHEVAL1 LC). specialize (IHEVAL2 LC).
+    inv IHEVAL1. repeat econstructor; eauto.
+  - apply IHEVAL2. exploit IHEVAL1; eauto.
+    intros LC'. inv LC'. auto.
+  - apply IHEVAL2. exploit IHEVAL1; eauto.
+    intros LC'. inv LC'. econstructor; eauto.
+  - repeat constructor.
+  - assert (wvalue (wvl_recv v1)).
+    + econstructor. instantiate (1 := L).
+      intros.
+      assert (env (nv_floc x ℓ σ)).
+      repeat (econstructor; eauto).
+      auto.
+    + repeat (constructor; auto).
+      exploit IHEVAL.
+      repeat (constructor; auto).
+      intro LC'.
+      inv LC'. auto.
+  - assert (wvalue (wvl_recv v1)).
+    + econstructor. instantiate (1 := L).
+      intros.
+      assert (env (nv_floc x ℓ σ)).
+      repeat (econstructor; eauto).
+      auto.
+    + repeat (constructor; auto).
+      exploit IHEVAL.
+      repeat (constructor; auto).
+      intro LC'.
+      inv LC'. auto.
+Qed.
+
+Lemma Eval_subst_loc {var loc} `{Eq var} `{Name loc} t (σ : nv var loc (@val var)) v (EVAL : Eval σ t v) :
+  forall ν ℓ', Eval (subst_loc_nv ν ℓ' σ) t (subst_loc_vl ν ℓ' v).
+Proof.
+  induction EVAL; ii; ss;
+  try solve [econstructor; eauto].
+  - econstructor 1.
+    erewrite read_env_subst_loc; eauto.
+    ss.
+  - assert (open_wvl_subst_loc_vl _ _ _ v) by (eapply open_wvl_subst_loc; auto).
+    rw; eauto.
+    econstructor 2.
+    erewrite read_env_subst_loc; eauto.
+    ss.
+  - eapply Ev_bind; eauto.
+    instantiate (1 := ℓ' :: L).
+    ii. split_nIn.
+    match goal with
+    | IH : forall _, ~ In _ ?L -> _, nIN : ~ In ?ν ?L |- _ =>
+      exploit (IH ν nIN)
+    end.
+    instantiate (1 := ℓ'). instantiate (1 := ν).
+    rewrite <- eqb_neq in nIN.
+    rw.
+    assert (open_loc_subst_loc_vl _ _ _ v1) by eapply open_loc_subst_loc.
+    rw. rw. auto.
+  - eapply Ev_bindevent; eauto.
+    instantiate (1 := ℓ' :: L).
+    ii. split_nIn.
+    match goal with
+    | IH : forall _, ~ In _ ?L -> _, nIN : ~ In ?ν ?L |- _ =>
+      exploit (IH ν nIN)
+    end.
+    instantiate (1 := ℓ'). instantiate (1 := ν).
+    rewrite <- eqb_neq in nIN.
+    rw.
+    assert (open_loc_subst_loc_vl _ _ _ v1) by eapply open_loc_subst_loc.
+    rw. rw. auto.
+Qed.
+
+Lemma Eval_subst_wvl {var loc} `{Eq var} `{Name loc} t (σ : nv var loc (@val var)) v (EVAL : Eval σ t v) :
+  forall u (U : wvalue u) ℓ', Eval (subst_wvl_nv u ℓ' σ) t (subst_wvl_vl u ℓ' v).
+Proof.
+  induction EVAL; ii; ss;
+  try solve [econstructor; eauto].
+  - econstructor 1.
+    erewrite read_env_subst_wvl; eauto.
+    ss.
+  - assert (open_wvl_subst_wvl_vl _ _ _ v) by (eapply open_wvl_subst_wvl; auto).
+    rw; eauto.
+    econstructor 2.
+    erewrite read_env_subst_wvl; eauto.
+    ss.
+  - eapply Ev_bind; eauto.
+    instantiate (1 := ℓ' :: L).
+    ii. split_nIn.
+    match goal with
+    | IH : forall _, ~ In _ ?L -> _, nIN : ~ In ?ν ?L |- _ =>
+      exploit (IH ν nIN); eauto
+    end.
+    instantiate (1 := ℓ').
+    des_goal; eqb2eq loc; clarify.
+    assert (open_loc_subst_wvl_vl _ _ _ v1) by (eapply open_loc_subst_wvl; eauto).
+    rw; eauto.
+  - eapply Ev_bindevent; eauto.
+    instantiate (1 := ℓ' :: L).
+    ii. split_nIn.
+    match goal with
+    | IH : forall _, ~ In _ ?L -> _, nIN : ~ In ?ν ?L |- _ =>
+      exploit (IH ν nIN); eauto
+    end.
+    instantiate (1 := ℓ').
+    des_goal; eqb2eq loc; clarify.
+    assert (open_loc_subst_wvl_vl _ _ _ v1) by (eapply open_loc_subst_wvl; eauto).
+    rw; eauto.
+Qed.
+
